src/Imps/Imp_resultis.v
@@ -96,9 +96,6 @@ with CEval : Com -> State -> State -> Prop :=
 
 #[global] Hint Constructors AEval BEval CEval : core.
 
-Ltac inv H :=
-  inversion H; subst; clear H; auto.
-
 Lemma AEval_det :
   forall {a : AExp} {s : State} {n m : nat},
     AEval a s n -> AEval a s m -> n = m
@@ -111,28 +108,32 @@ with CEval_det :
   forall (c : Com) (s s1 : State),
     CEval c s s1 -> forall s2 : State, CEval c s s2 -> s1 = s2.
 Proof.
-  - destruct 1; intros * HI *; inv HI.
-    + rewrite (AEval_det _ _ _ _ H H3), (AEval_det _ _ _ _ H0 H6). reflexivity.
-    + rewrite (AEval_det _ _ _ _ H H3), (AEval_det _ _ _ _ H0 H6). reflexivity.
-    + rewrite (AEval_det _ _ _ _ H H3), (AEval_det _ _ _ _ H0 H6). reflexivity.
-    + specialize (CEval_det _ _ _ H _ H3). subst.
-       rewrite (AEval_det _ _ _ _ H0 H6). reflexivity.
-  - destruct 1; intros * HI *; inv HI.
-    + rewrite (AEval_det _ _ _ _ H H3), (AEval_det _ _ _ _ H0 H6). reflexivity.
-    + rewrite (AEval_det _ _ _ _ H H3), (AEval_det _ _ _ _ H0 H6). reflexivity.
-    + rewrite (BEval_det _ _ _ H _ H1). reflexivity.
-    + rewrite (BEval_det _ _ _ H _ H3), (BEval_det _ _ _ H0 _ H6). reflexivity.
-    + rewrite (BEval_det _ _ _ H _ H3), (BEval_det _ _ _ H0 _ H6). reflexivity.
-  - destruct 1; intros * HI *; inv HI.
-    + rewrite (AEval_det _ _ _ _ H H4). reflexivity.
-    + destruct (CEval_det _ _ _ H _ H3), (CEval_det _ _ _ H0 _ H6). reflexivity.
-    + rewrite (CEval_det _ _ _ H0 _ H7). reflexivity.
-    + specialize (BEval_det _ _ _ H _ H6). congruence.
-    + specialize (BEval_det _ _ _ H _ H6). congruence.
-    + rewrite (CEval_det _ _ _ H0 _ H7). reflexivity.
-    + specialize (BEval_det _ _ _ H _ H2). congruence.
-    + specialize (BEval_det _ _ _ H _ H6). congruence.
-    + destruct (CEval_det _ _ _ H0 _ H5), (CEval_det _ _ _ H1 _ H8). reflexivity.
+  - destruct 1; intros * HI *; inversion HI; subst; try now auto.
+    + now eapply AEval_det in H3 as <-, H6 as <-.
+    + now eapply AEval_det in H3 as <-, H6 as <-.
+    + now eapply AEval_det in H3 as <-, H6 as <-.
+    + specialize (CEval_det _ _ _ H _ H3) as ->.
+      now eapply AEval_det in H6 as <-.
+  - destruct 1; intros * HI *; inversion HI; subst; try now auto.
+    + now eapply AEval_det in H3 as <-, H6 as <-.
+    + now eapply AEval_det in H3 as <-, H6 as <-.
+    + now eapply BEval_det in H1 as <-.
+    + now now eapply BEval_det in H3 as <-, H6 as <-.
+    + now eapply BEval_det in H3 as <-, H6 as <-.
+  - destruct 1; intros * HI *; inversion HI; subst; try now auto.
+    + now eapply AEval_det in H4 as <-.
+    + now destruct (CEval_det _ _ _ H _ H3), (CEval_det _ _ _ H0 _ H6).
+    + now eapply CEval_det in H7 as <-.
+    + cut (false = true); [easy |].
+      now eapply BEval_det; eauto.
+    + cut (true = false); [easy |].
+      now eapply BEval_det; eauto.
+    + now eapply CEval_det; eauto.
+    + cut (false = true); [easy |].
+      now eapply BEval_det; eauto.
+    + cut (true = false); [easy |].
+      now eapply BEval_det; eauto.
+    + now destruct (CEval_det _ _ _ H0 _ H5), (CEval_det _ _ _ H1 _ H8).
 Qed.
 
 Set Warnings "-funind-cannot-define-graph".
@@ -207,29 +208,28 @@ with ceval_CEval (fuel : nat) :
   forall {c : Com} {s1 s2 : State},
     ceval fuel c s1 = Some s2 -> CEval c s1 s2.
 Proof.
-  - destruct fuel as [| fuel']; cbn; intros.
-    + easy.
-    + destruct a; [now inv H | now inv H |
-        now destruct (aeval fuel' a1 s) eqn: H1, (aeval fuel' a2 s) eqn: H2; inv H; eauto.. |].
-      now destruct (ceval fuel' c s) eqn: H1; inv H; eauto.
-  - destruct fuel as [| fuel']; cbn; intros.
-    + easy.
-    + destruct e.
-      * now inv H.
-      * now inv H.
-      * now destruct (aeval fuel' a s) eqn: H1, (aeval fuel' a0 s) eqn: H2; inv H; eauto.
-      * now destruct (aeval fuel' a s) eqn: H1, (aeval fuel' a0 s) eqn: H2; inv H; eauto.
-      * now destruct (beval fuel' e s) eqn: H1; inv H; eauto.
-      * now destruct (beval fuel' e1 s) eqn: H1, (beval fuel' e2 s) eqn: H2; inv H; eauto.
-      * now destruct (beval fuel' e1 s) eqn: H1, (beval fuel' e2 s) eqn: H2; inv H; eauto.
+  - destruct fuel as [| fuel']; cbn; intros; [easy |].
+    destruct a; [now inversion H | now inversion H |
+      now destruct (aeval fuel' a1 s) eqn: H1, (aeval fuel' a2 s) eqn: H2;
+        inversion H; subst; clear H; eauto.. |].
+    now destruct (ceval fuel' c s) eqn: H1; inversion H; subst; clear H; eauto.
+  - destruct fuel as [| fuel']; cbn; intros; [easy |].
+    destruct e.
+    + now injection H as [= <-]; constructor.
+    + now injection H as [= <-]; constructor.
+    + now destruct (aeval fuel' a s) eqn: H1, (aeval fuel' a0 s) eqn: H2; inversion H; subst; eauto.
+    + now destruct (aeval fuel' a s) eqn: H1, (aeval fuel' a0 s) eqn: H2; inversion H; subst; eauto.
+    + now destruct (beval fuel' e s) eqn: H1; inversion H; subst; eauto.
+    + now destruct (beval fuel' e1 s) eqn: H1, (beval fuel' e2 s) eqn: H2; inversion H; subst; eauto.
+    + now destruct (beval fuel' e1 s) eqn: H1, (beval fuel' e2 s) eqn: H2; inversion H; subst; eauto.
   - destruct fuel as [| fuel']; cbn; intros; [easy |].
     destruct c.
-    * now inversion H; subst; constructor.
-    * now destruct (aeval fuel' a0 s1) eqn: H1; inv H; eauto.
-    * now destruct (ceval fuel' c1 s1) eqn: H1; inv H; eauto.
-    * destruct (beval fuel' b s1) eqn: H1; [| easy].
+    + now inversion H; subst; constructor.
+    + now destruct (aeval fuel' a0 s1) eqn: H1; inversion H; subst; eauto.
+    + now destruct (ceval fuel' c1 s1) eqn: H1; inversion H; subst; eauto.
+    + destruct (beval fuel' b s1) eqn: H1; [| easy].
       now destruct b0; eauto.
-    * destruct (beval fuel' b s1) eqn: H1; [| easy].
-      destruct b0; inv H; eauto.
-      now destruct (ceval fuel' c s1) eqn: H'; inv H1; eauto.
+    + destruct (beval fuel' b s1) eqn: H1; [| easy].
+      destruct b0; inversion H; subst; eauto.
+      now destruct (ceval fuel' c s1) eqn: H'; inversion H1; subst; eauto.
 Qed.
